@prefix :        <http://purl.org/ontology/bibo/> .
@prefix ns:      <http://www.w3.org/2003/06/sw-vocab-status/ns#> .
@prefix foaf:    <http://xmlns.com/foaf/0.1/> .
@prefix status:  <http://purl.org/ontology/bibo/status/> .
@prefix terms:   <http://purl.org/dc/terms/> .
@prefix vann:    <http://purl.org/vocab/vann/> .
@prefix degrees:  <http://purl.org/ontology/bibo/degrees/> .
@prefix schema:  <http://schemas.talis.com/2005/address/schema#> .
@prefix rdfs:    <http://www.w3.org/2000/01/rdf-schema#> .
@prefix event:   <http://purl.org/NET/c4dm/event.owl#> .
@prefix bibo:    <http://purl.org/ontology/bibo/> .
@prefix xsd:     <http://www.w3.org/2001/XMLSchema#> .
@prefix owl:     <http://www.w3.org/2002/07/owl#> .
@prefix rdf:     <http://www.w3.org/1999/02/22-rdf-syntax-ns#> .
@prefix skos:    <http://www.w3.org/2004/02/skos/core#> .
@prefix prism:   <http://prismstandard.org/namespaces/1.2/basic/> .

ns:term_status
      a       owl:AnnotationProperty .

bibo:volume
      a       owl:DatatypeProperty ;
      rdfs:comment "A volume number"@en ;
      rdfs:domain bibo:Document ;
      rdfs:isDefinedBy "http://purl.org/ontology/bibo/"^^xsd:anyURI ;
      rdfs:label "volume"@en ;
      rdfs:range rdfs:Literal ;
      rdfs:subPropertyOf bibo:locator ;
      ns:term_status "stable" .

bibo:abstract
      a       owl:DatatypeProperty ;
      rdfs:comment "A summary of the resource." ;
      rdfs:domain rdfs:Resource ;
      rdfs:isDefinedBy "http://purl.org/ontology/bibo/"^^xsd:anyURI ;
      rdfs:label "abstract" ;
      rdfs:range rdfs:Literal ;
      ns:term_status "stable" .

event:produced_in
      a       owl:ObjectProperty .

bibo:Note
      a       owl:Class ;
      rdfs:comment "Notes or annotations about a resource."@en ;
      rdfs:isDefinedBy "http://purl.org/ontology/bibo/"^^xsd:anyURI ;
      rdfs:label "Note"@en ;
      rdfs:subClassOf bibo:Document ;
      ns:term_status "stable" .

bibo:argued
      a       owl:DatatypeProperty ;
      rdfs:comment "The date on which a legal case is argued before a court. Date is of format xsd:date"@en ;
      rdfs:domain bibo:LegalDocument ;
      rdfs:isDefinedBy "http://purl.org/ontology/bibo/"^^xsd:anyURI ;
      rdfs:label "date argued"@en ;
      rdfs:range rdfs:Literal ;
      ns:term_status "unstable" .

event:sub_event
      a       owl:ObjectProperty ;
      skos:scopeNote "Used to link big events with smaller events such as workshops that happen in the context of a conference."@en .

status:accepted
      a       bibo:DocumentStatus , owl:Thing , owl:NamedIndividual ;
      rdfs:comment "Accepted for publication after peer reviewing."@en ;
      rdfs:label "accepted"@en ;
      ns:term_status "stable" .

bibo:fgiasson
      a       foaf:Person , owl:Thing , owl:NamedIndividual ;
      rdfs:isDefinedBy "http://purl.org/ontology/bibo/"^^xsd:anyURI ;
      rdfs:seeAlso "http://fgiasson.com/me/"^^xsd:anyURI ;
      foaf:name "Frederick Giasson" .

bibo:section
      a       owl:DatatypeProperty ;
      rdfs:comment "A section number"@en ;
      rdfs:domain bibo:Document ;
      rdfs:isDefinedBy "http://purl.org/ontology/bibo/"^^xsd:anyURI ;
      rdfs:label "section"@en ;
      rdfs:range rdfs:Literal ;
      rdfs:subPropertyOf bibo:locator ;
      ns:term_status "unstable" ;
      skos:example """Di Rado, Alicia. 1995. Trekking through college: Classes explore
modern society using the world of Star trek. Los Angeles Times, March
15, sec. A, p. 3."""@en .

degrees:ms
      a       owl:Thing , owl:NamedIndividual , bibo:ThesisDegree ;
      rdfs:comment "masters degree in science"@en ;
      rdfs:label "M.S."@en ;
      ns:term_status "stable" .

terms:format
      a       owl:ObjectProperty ;
      skos:example """<dcterms:format>
   <dcterms:MediaTypeOrExtent>
     <rdf:value>text/html</rdf:value>
     <rdfs:label>HTML</rdfs:label>
   </dcterms:MediaTypeOrExtent>
 </dcterms:format>"""@en ;
      skos:scopeNote "Used to describe the format of a bibliographic resource."@en .

bibo:issue
      a       owl:DatatypeProperty ;
      rdfs:comment "An issue number"@en ;
      rdfs:domain bibo:Issue ;
      rdfs:isDefinedBy "http://purl.org/ontology/bibo/"^^xsd:anyURI ;
      rdfs:label "issue"@en ;
      rdfs:range rdfs:Literal ;
      rdfs:subPropertyOf bibo:locator ;
      ns:term_status "stable" .

terms:isReferencedBy
      a       owl:ObjectProperty ;
      skos:scopeNote "Used to relate a reference citation to a bibliographic resource."@en .

bibo:interviewer
      a       owl:ObjectProperty ;
      rdfs:comment "An agent that interview another agent."@en ;
      rdfs:domain foaf:Agent ;
      rdfs:isDefinedBy "http://purl.org/ontology/bibo/"^^xsd:anyURI ;
      rdfs:label "interviewer" ;
      rdfs:range foaf:Agent ;
      rdfs:subPropertyOf terms:contributor ;
      ns:term_status "stable" .

bibo:chapter
      a       owl:DatatypeProperty ;
      rdfs:comment "An chapter number"@en ;
      rdfs:domain bibo:BookSection ;
      rdfs:isDefinedBy "http://purl.org/ontology/bibo/"^^xsd:anyURI ;
      rdfs:label "chapter"@en ;
      rdfs:range rdfs:Literal ;
      rdfs:subPropertyOf bibo:locator ;
      ns:term_status "unstable" .

bibo:number
      a       owl:DatatypeProperty ;
      rdfs:comment "A generic item or document number. Not to be confused with issue number."@en ;
      rdfs:domain bibo:Document ;
      rdfs:isDefinedBy "http://purl.org/ontology/bibo/"^^xsd:anyURI ;
      rdfs:label "number"@en ;
      rdfs:range rdfs:Literal ;
      ns:term_status "stable" .

terms:isVersionOf
      a       owl:ObjectProperty .

bibo:Email
      a       owl:Class ;
      rdfs:comment "A written communication addressed to a person or organization and transmitted electronically."@en ;
      rdfs:isDefinedBy "http://purl.org/ontology/bibo/"^^xsd:anyURI ;
      rdfs:label "EMail"@en ;
      rdfs:subClassOf bibo:PersonalCommunicationDocument ;
      ns:term_status "stable" .

terms:created
      a       owl:DatatypeProperty ;
      rdfs:subPropertyOf terms:date ;
      skos:scopeNote "Used to describe the creation date of a bibliographic item"@en .

terms:creator
      a       owl:AnnotationProperty .

degrees:phd
      a       owl:Thing , owl:NamedIndividual , bibo:ThesisDegree ;
      rdfs:comment "PhD degree"@en ;
      rdfs:label "PhD degree"@en ;
      ns:term_status "stable" .

prism:issn
      a       owl:DatatypeProperty ;
      owl:equivalentProperty
              bibo:issn .

bibo:sici
      a       owl:DatatypeProperty ;
      rdfs:domain
              [ a       owl:Class ;
                owl:unionOf (bibo:Collection bibo:Document)
              ] ;
      rdfs:range rdfs:Literal ;
      rdfs:subPropertyOf bibo:identifier .

skos:historyNote
      a       owl:AnnotationProperty .

bibo:issn
      a       owl:DatatypeProperty ;
      rdfs:domain bibo:Collection ;
      rdfs:range rdfs:Literal ;
      rdfs:subPropertyOf bibo:identifier .

bibo:Patent
      a       owl:Class ;
      rdfs:comment "A document describing the exclusive right granted by a government to an inventor to manufacture, use, or sell an invention for a certain number of years."@en ;
      rdfs:isDefinedBy "http://purl.org/ontology/bibo/"^^xsd:anyURI ;
      rdfs:label "Patent"@en ;
      rdfs:subClassOf bibo:Document ;
      ns:term_status "stable" .

bibo:Journal
      a       owl:Class ;
      rdfs:comment "A periodical of scholarly journal Articles."@en ;
      rdfs:isDefinedBy "http://purl.org/ontology/bibo/"^^xsd:anyURI ;
      rdfs:label "Journal"@en ;
      rdfs:subClassOf bibo:Periodical ;
      rdfs:subClassOf
              [ a       owl:Restriction ;
                owl:minCardinality "1"^^xsd:nonNegativeInteger ;
                owl:onProperty terms:hasPart
              ] ;
      rdfs:subClassOf
              [ a       owl:Restriction ;
                owl:allValuesFrom bibo:Issue ;
                owl:onProperty terms:hasPart
              ] ;
      ns:term_status "stable" .

bibo:Newspaper
      a       owl:Class ;
      rdfs:comment "A periodical of documents, usually issued daily or weekly, containing current news, editorials, feature articles, and usually advertising."@en ;
      rdfs:isDefinedBy "http://purl.org/ontology/bibo/"^^xsd:anyURI ;
      rdfs:label "Newspaper"@en ;
      rdfs:subClassOf bibo:Periodical ;
      rdfs:subClassOf
              [ a       owl:Restriction ;
                owl:minCardinality "1"^^xsd:nonNegativeInteger ;
                owl:onProperty terms:hasPart
              ] ;
      rdfs:subClassOf
              [ a       owl:Restriction ;
                owl:allValuesFrom bibo:Issue ;
                owl:onProperty terms:hasPart
              ] ;
      ns:term_status "stable" .

bibo:CourtReporter
      a       owl:Class ;
      rdfs:comment "A collection of legal cases."@en ;
      rdfs:isDefinedBy "http://purl.org/ontology/bibo/"^^xsd:anyURI ;
      rdfs:label "Court Reporter"@en ;
      rdfs:subClassOf bibo:Periodical ;
      rdfs:subClassOf
              [ a       owl:Restriction ;
                owl:minCardinality "1"^^xsd:nonNegativeInteger ;
                owl:onProperty terms:hasPart
              ] ;
      rdfs:subClassOf
              [ a       owl:Restriction ;
                owl:allValuesFrom bibo:LegalDocument ;
                owl:onProperty terms:hasPart
              ] ;
      ns:term_status "stable" .

foaf:based_near
      a       owl:ObjectProperty ;
      skos:scopeNote "Used to link an agent, related to bibliographic things, to a place where it is based near: can be a city, a monument, a building, etc."@en .

event:product
      a       owl:ObjectProperty ;
      skos:scopeNote "Used to link an event such as a conference to an outcome (a product) of that event, for example, an article, a proceeding, etc."@en .

foaf:Person
      a       owl:Class ;
      skos:scopeNote "Used to describe a Person related to a bibliographic ite such as an author, an editor, etc."@en .

degrees:ma
      a       owl:Thing , owl:NamedIndividual , bibo:ThesisDegree ;
      rdfs:comment "masters degree in arts"@en ;
      rdfs:label "M.A."@en ;
      ns:term_status "stable" .

bibo:pageStart
      a       owl:DatatypeProperty ;
      rdfs:comment "Starting page number within a continuous page range."@en ;
      rdfs:domain bibo:Document ;
      rdfs:isDefinedBy "http://purl.org/ontology/bibo/"^^xsd:anyURI ;
      rdfs:label "page start"@en ;
      rdfs:range rdfs:Literal ;
      rdfs:subPropertyOf bibo:locator ;
      ns:term_status "stable" .

terms:publisher
      a       owl:ObjectProperty ;
      skos:scopeNote "Used to link a bibliographic item to its publisher."@en .

status:draft
      a       bibo:DocumentStatus , owl:Thing , owl:NamedIndividual ;
      rdfs:comment "Document drafted"@en ;
      rdfs:label "draft"@en ;
      ns:term_status "stable" .

bibo:Slideshow
      a       owl:Class ;
      rdfs:comment "A presentation of a series of slides, usually presented in front of an audience with written text and images."@en ;
      rdfs:isDefinedBy "http://purl.org/ontology/bibo/"^^xsd:anyURI ;
      rdfs:label "Slideshow"@en ;
      rdfs:subClassOf bibo:Document ;
      rdfs:subClassOf
              [ a       owl:Restriction ;
                owl:allValuesFrom bibo:Slide ;
                owl:onProperty terms:hasPart
              ] ;
      ns:term_status "stable" .

foaf:givenname
      a       owl:DatatypeProperty ;
      skos:scopeNote "This is the property we choose to describe the given name of a Person related to a bibliographic resource. This is the first name of a person."@en .

bibo:prefixName
      a       owl:DatatypeProperty ;
      rdfs:comment "The prefix of a name"@en ;
      rdfs:domain foaf:Agent ;
      rdfs:isDefinedBy "http://purl.org/ontology/bibo/"^^xsd:anyURI ;
      rdfs:label "prefix name"@en ;
      rdfs:range rdfs:Literal ;
      ns:term_status "stable" .

rdfs:Resource
      a       owl:Class .

skos:example
      a       owl:AnnotationProperty .

terms:references
      a       owl:ObjectProperty .

bibo:recipient
      a       owl:ObjectProperty ;
      rdfs:comment "An agent that receives a communication document."@en ;
      rdfs:domain bibo:PersonalCommunicationDocument ;
      rdfs:isDefinedBy "http://purl.org/ontology/bibo/"^^xsd:anyURI ;
      rdfs:label "recipient" ;
      rdfs:range foaf:Agent ;
      ns:term_status "stable" .

status:rejected
      a       bibo:DocumentStatus , owl:Thing , owl:NamedIndividual ;
      rdfs:comment "Rejected for publication after peer reviewing."@en ;
      rdfs:label "rejected"@en ;
      ns:term_status "stable" .

bibo:Slide
      a       owl:Class ;
      rdfs:comment "A slide in a slideshow"@en ;
      rdfs:isDefinedBy "http://purl.org/ontology/bibo/"^^xsd:anyURI ;
      rdfs:label "Slide"@en ;
      rdfs:subClassOf bibo:DocumentPart ;
      ns:term_status "unstable" .

bibo:Manuscript
      a       owl:Class ;
      rdfs:comment "An unpublished Document, which may also be submitted to a publisher for publication."@en ;
      rdfs:isDefinedBy "http://purl.org/ontology/bibo/"^^xsd:anyURI ;
      rdfs:label "Manuscript"@en ;
      rdfs:subClassOf bibo:Document ;
      ns:term_status "stable" .

bibo:Excerpt
      a       owl:Class ;
      rdfs:comment "A passage selected from a larger work."@en ;
      rdfs:isDefinedBy "http://purl.org/ontology/bibo/"^^xsd:anyURI ;
      rdfs:label "Excerpt"@en ;
      rdfs:subClassOf bibo:DocumentPart ;
      ns:term_status "stable" .

rdf:List
      a       owl:Class .

status:legal
      a       bibo:DocumentStatus , owl:Thing , owl:NamedIndividual ;
      rdfs:comment "Legal document"@en ;
      rdfs:label "legal"@en ;
      ns:term_status "stable" .

bibo:Code
      a       owl:Class ;
      rdfs:comment "A collection of statutes."@en ;
      rdfs:isDefinedBy "http://purl.org/ontology/bibo/"^^xsd:anyURI ;
      rdfs:label "Code"@en ;
      rdfs:subClassOf bibo:Periodical ;
      rdfs:subClassOf
              [ a       owl:Restriction ;
                owl:minCardinality "1"^^xsd:nonNegativeInteger ;
                owl:onProperty terms:hasPart
              ] ;
      rdfs:subClassOf
              [ a       owl:Restriction ;
                owl:allValuesFrom bibo:Legislation ;
                owl:onProperty terms:hasPart
              ] ;
      ns:term_status "stable" .

bibo:annotates
      a       owl:ObjectProperty ;
      rdfs:comment "Critical or explanatory note for a Document."@en ;
      rdfs:domain bibo:Note ;
      rdfs:isDefinedBy "http://purl.org/ontology/bibo/"^^xsd:anyURI ;
      rdfs:label "annotates"@en ;
      rdfs:range rdfs:Resource ;
      rdfs:subPropertyOf terms:relation ;
      ns:term_status "stable" .

foaf:homepage
      a       owl:ObjectProperty ;
      skos:scopeNote "Used to link an agent to its homepage (which is a web page accessible using a URL)."@en .

skos:editorialNote
      a       owl:AnnotationProperty .

bibo:pages
      a       owl:DatatypeProperty ;
      rdfs:comment "A string of non-contiguous page spans that locate a Document within a Collection. Example: 23-25, 34, 54-56. For continuous page ranges, use the pageStart and pageEnd properties."@en ;
      rdfs:domain bibo:Document ;
      rdfs:isDefinedBy "http://purl.org/ontology/bibo/"^^xsd:anyURI ;
      rdfs:label "pages"@en ;
      rdfs:range rdfs:Literal ;
      rdfs:subPropertyOf bibo:locator ;
      ns:term_status "stable" .

rdf:value
      a       owl:ObjectProperty ;
      skos:scopeNote """Used to describe the content of a bibo:Document and othr bibliographic resouces.

We suggest to use this property instead of the deprecated \"bibo:content\" one."""@en .

bibo:reversedBy
      a       owl:ObjectProperty ;
      rdfs:comment "A legal decision that reverses a ruling."@en ;
      rdfs:domain bibo:LegalDecision ;
      rdfs:isDefinedBy "http://purl.org/ontology/bibo/"^^xsd:anyURI ;
      rdfs:range bibo:LegalDecision ;
      rdfs:subPropertyOf bibo:subsequentLegalDecision .

bibo:Performance
      a       owl:Class ;
      rdfs:comment "A public performance."@en ;
      rdfs:isDefinedBy "http://purl.org/ontology/bibo/"^^xsd:anyURI ;
      rdfs:label "Performance"@en ;
      rdfs:subClassOf event:Event ;
      ns:term_status "unstable" .

bibo:identifier
      a       owl:DatatypeProperty ;
      rdfs:domain
              [ a       owl:Class ;
                owl:unionOf (bibo:Collection bibo:Document)
              ] ;
      rdfs:range rdfs:Literal .

bibo:upc
      a       owl:DatatypeProperty ;
      rdfs:domain
              [ a       owl:Class ;
                owl:unionOf (bibo:Collection bibo:Document)
              ] ;
      rdfs:range rdfs:Literal ;
      rdfs:subPropertyOf bibo:identifier .

bibo:reviewOf
      a       owl:ObjectProperty ;
      rdfs:comment "Relates a review document to a reviewed thing (resource, item, etc.)."@en ;
      rdfs:domain bibo:Document ;
      rdfs:isDefinedBy "http://purl.org/ontology/bibo/"^^xsd:anyURI ;
      rdfs:label "review of"@en ;
      rdfs:range rdfs:Resource ;
      rdfs:subPropertyOf terms:relation ;
      ns:term_status "stable" .

bibo:Letter
      a       owl:Class ;
      rdfs:comment "A written or printed communication addressed to a person or organization and usually transmitted by mail."@en ;
      rdfs:isDefinedBy "http://purl.org/ontology/bibo/"^^xsd:anyURI ;
      rdfs:label "Letter"@en ;
      rdfs:subClassOf bibo:PersonalCommunicationDocument ;
      ns:term_status "stable" .

status:published
      a       bibo:DocumentStatus , owl:Thing , owl:NamedIndividual ;
      rdfs:comment "Published document"@en ;
      rdfs:label "published"@en ;
      ns:term_status "stable" .

skos:note
      a       owl:AnnotationProperty .

bibo:Website
      a       owl:Class ;
      rdfs:comment "A group of Webpages accessible on the Web."@en ;
      rdfs:isDefinedBy "http://purl.org/ontology/bibo/"^^xsd:anyURI ;
      rdfs:label "Website"@en ;
      rdfs:subClassOf bibo:Collection ;
      rdfs:subClassOf
              [ a       owl:Restriction ;
                owl:minCardinality "1"^^xsd:nonNegativeInteger ;
                owl:onProperty terms:hasPart
              ] ;
      rdfs:subClassOf
              [ a       owl:Restriction ;
                owl:allValuesFrom bibo:Webpage ;
                owl:onProperty terms:hasPart
              ] ;
      ns:term_status "unstable" .

skos:scopeNote
      a       owl:AnnotationProperty .

bibo:CollectedDocument
      a       owl:Class ;
      rdfs:comment "A document that simultaneously contains other documents."@en ;
      rdfs:isDefinedBy "http://purl.org/ontology/bibo/"^^xsd:anyURI ;
      rdfs:label "Collected Document"@en ;
      rdfs:subClassOf bibo:Document ;
      rdfs:subClassOf
              [ a       owl:Restriction ;
                owl:allValuesFrom bibo:Document ;
                owl:onProperty terms:hasPart
              ] ;
      rdfs:subClassOf
              [ a       owl:Restriction ;
                owl:minCardinality "1"^^xsd:nonNegativeInteger ;
                owl:onProperty terms:hasPart
              ] ;
      ns:term_status "stable" .

bibo:Issue
      a       owl:Class ;
      rdfs:comment "something that is printed or published and distributed, esp. a given number of a periodical"@en ;
      rdfs:isDefinedBy "http://purl.org/ontology/bibo/"^^xsd:anyURI ;
      rdfs:label "Issue"@en ;
      rdfs:subClassOf bibo:CollectedDocument ;
      rdfs:subClassOf
              [ a       owl:Restriction ;
                owl:allValuesFrom bibo:Article ;
                owl:onProperty terms:hasPart
              ] ;
      rdfs:subClassOf
              [ a       owl:Restriction ;
                owl:minCardinality "1"^^xsd:nonNegativeInteger ;
                owl:onProperty terms:hasPart
              ] ;
      ns:term_status "stable" .

bibo:Event
      a       owl:Class .

owl:deprecated
      a       owl:AnnotationProperty .

bibo:director
      a       owl:ObjectProperty ;
      rdfs:comment "A Film director."@en ;
      rdfs:domain bibo:AudioVisualDocument ;
      rdfs:isDefinedBy "http://purl.org/ontology/bibo/"^^xsd:anyURI ;
      rdfs:label "director" ;
      rdfs:range foaf:Agent ;
      rdfs:subPropertyOf terms:contributor ;
      ns:term_status "stable" .

foaf:Agent
      a       owl:Class ;
      skos:scopeNote "Used to describe any \"agent\" related to bibliographic items. Such agents can be persons, organizations or groups of any kind."@en .

skos:changeNote
      a       owl:AnnotationProperty .

bibo:ThesisDegree
      a       owl:Class ;
      rdfs:comment "The academic degree of a Thesis"@en ;
      rdfs:isDefinedBy "http://purl.org/ontology/bibo/"^^xsd:anyURI ;
      rdfs:label "Thesis degree"@en ;
      ns:term_status "stable" .

bibo:Magazine
      a       owl:Class ;
      rdfs:comment "A periodical of magazine Articles. A magazine is a publication that is issued periodically, usually bound in a paper cover, and typically contains essays, stories, poems, etc., by many writers, and often photographs and drawings, frequently specializing in a particular subject or area, as hobbies, news, or sports."@en ;
      rdfs:isDefinedBy "http://purl.org/ontology/bibo/"^^xsd:anyURI ;
      rdfs:label "Magazine"@en ;
      rdfs:subClassOf bibo:Periodical ;
      rdfs:subClassOf
              [ a       owl:Restriction ;
                owl:allValuesFrom bibo:Issue ;
                owl:onProperty terms:hasPart
              ] ;
      rdfs:subClassOf
              [ a       owl:Restriction ;
                owl:minCardinality "1"^^xsd:nonNegativeInteger ;
                owl:onProperty terms:hasPart
              ] ;
      ns:term_status "stable" .

bibo:handle
      a       owl:DatatypeProperty ;
      rdfs:domain
              [ a       owl:Class ;
                owl:unionOf (bibo:Collection bibo:Document)
              ] ;
      rdfs:range rdfs:Literal ;
      rdfs:subPropertyOf bibo:identifier .

terms:title
      a       owl:AnnotationProperty , owl:ObjectProperty ;
      skos:scopeNote "Used to describe the title of a bibliographic resource"@en .

bibo:authorList
      a       owl:ObjectProperty ;
      rdfs:comment "An ordered list of authors. Normally, this list is seen as a priority list that order authors by importance."@en ;
      rdfs:domain bibo:Document ;
      rdfs:isDefinedBy "http://purl.org/ontology/bibo/"^^xsd:anyURI ;
      rdfs:label "list of authors"@en ;
      rdfs:range
              [ a       owl:Class ;
                owl:unionOf (rdf:List rdf:Seq)
              ] ;
      rdfs:subPropertyOf bibo:contributorList ;
      ns:term_status "stable" .

bibo:Thesis
      a       owl:Class ;
      rdfs:comment "A document created to summarize research findings associated with the completion of an academic degree."@en ;
      rdfs:isDefinedBy "http://purl.org/ontology/bibo/"^^xsd:anyURI ;
      rdfs:label "Thesis"@en ;
      rdfs:subClassOf bibo:Document ;
      ns:term_status "stable" .

bibo:owner
      a       owl:ObjectProperty ;
      rdfs:comment "Owner of a document or a collection of documents."@en ;
      rdfs:domain
              [ a       owl:Class ;
                owl:unionOf (bibo:Collection bibo:Document)
              ] ;
      rdfs:isDefinedBy "http://purl.org/ontology/bibo/"^^xsd:anyURI ;
      rdfs:label "owner"@en ;
      rdfs:range foaf:Agent ;
      ns:term_status "unstable" .

status:unpublished
      a       bibo:DocumentStatus , owl:Thing , owl:NamedIndividual ;
      rdfs:comment "Unpublished document"@en ;
      rdfs:label "unpublished"@en ;
      ns:term_status "stable" .

terms:contributor
      a       owl:ObjectProperty ;
      skos:scopeNote "Used to link a bibliographic item to one of its contributor: can be an author, an editor, a publisher, etc."@en .

bibo:lccn
      a       owl:DatatypeProperty ;
      rdfs:domain
              [ a       owl:Class ;
                owl:unionOf (bibo:Collection bibo:Document)
              ] ;
      rdfs:range rdfs:Literal ;
      rdfs:subPropertyOf bibo:identifier .

event:agent
      a       owl:ObjectProperty ;
      skos:changeNote "Used to link an agent (a person) to an event (a conference, an hearing, etc.)"@en .

bibo:Workshop
      a       owl:Class ;
      rdfs:comment "A seminar, discussion group, or the like, that emphasizes zxchange of ideas and the demonstration and application of techniques, skills, etc."@en ;
      rdfs:isDefinedBy "http://purl.org/ontology/bibo/"^^xsd:anyURI ;
      rdfs:label "Workshop"@en ;
      rdfs:subClassOf event:Event ;
      ns:term_status "stable" .

event:time
      a       owl:ObjectProperty ;
      skos:scopeNote "Used to describe the timing of an event. For example, when a conference starts and stops."@en .

bibo:Map
      a       owl:Class ;
      rdfs:comment "A graphical depiction of geographic features."@en ;
      rdfs:isDefinedBy "http://purl.org/ontology/bibo/"^^xsd:anyURI ;
      rdfs:label "Map"@en ;
      rdfs:subClassOf bibo:Image ;
      ns:term_status "unstable" .

terms:isPartOf
      a       owl:ObjectProperty .

bibo:Conference
      a       owl:Class ;
      rdfs:comment "A meeting for consultation or discussion."@en ;
      rdfs:isDefinedBy "http://purl.org/ontology/bibo/"^^xsd:anyURI ;
      rdfs:label "Conference"@en ;
      rdfs:subClassOf event:Event ;
      ns:term_status "stable" .

terms:hasPart
      a       owl:ObjectProperty .

foaf:depiction
      a       owl:ObjectProperty ;
      skos:scopeNote "Used to link an agent with an image that depict it."@en .

bibo:pmid
      a       owl:DatatypeProperty ;
      rdfs:domain
              [ a       owl:Class ;
                owl:unionOf (bibo:Collection bibo:Document)
              ] ;
      rdfs:range rdfs:Literal ;
      rdfs:subPropertyOf bibo:identifier .

prism:endingPage
      a       owl:DatatypeProperty ;
      owl:equivalentProperty
              bibo:pageEnd .

bibo:Film
      a       owl:Class ;
      rdfs:comment "aka movie."@en ;
      rdfs:isDefinedBy "http://purl.org/ontology/bibo/"^^xsd:anyURI ;
      rdfs:label "Film"@en ;
      rdfs:subClassOf bibo:AudioVisualDocument ;
      ns:term_status "stable" .

bibo:Chapter
      a       owl:Class ;
      rdfs:comment "A chapter of a book."@en ;
      rdfs:isDefinedBy "http://purl.org/ontology/bibo/"^^xsd:anyURI ;
      rdfs:label "Chapter"@en ;
      rdfs:subClassOf bibo:BookSection ;
      ns:term_status "unstable" .

terms:identifier
      a       owl:AnnotationProperty .

status:nonPeerReviewed
      a       bibo:DocumentStatus , owl:Thing , owl:NamedIndividual ;
      rdfs:comment "A document that is not peer reviewed"@en ;
      rdfs:label "non peer reviewed"@en ;
      ns:term_status "stable" .

bibo:Periodical
      a       owl:Class ;
      rdfs:comment "A group of related documents issued at regular intervals."@en ;
      rdfs:isDefinedBy "http://purl.org/ontology/bibo/"^^xsd:anyURI ;
      rdfs:label "Periodical"@en ;
      rdfs:subClassOf bibo:Collection ;
      rdfs:subClassOf
              [ a       owl:Restriction ;
                owl:allValuesFrom bibo:Issue ;
                owl:onProperty terms:hasPart
              ] ;
      rdfs:subClassOf
              [ a       owl:Restriction ;
                owl:minCardinality "1"^^xsd:nonNegativeInteger ;
                owl:onProperty terms:hasPart
              ] ;
      ns:term_status "stable" .

bibo:MultiVolumeBook
      a       owl:Class ;
      rdfs:comment "A loose, thematic, collection of Documents, often Books."@en ;
      rdfs:isDefinedBy "http://purl.org/ontology/bibo/"^^xsd:anyURI ;
      rdfs:label "Multivolume Book"@en ;
      rdfs:subClassOf bibo:Collection ;
      rdfs:subClassOf
              [ a       owl:Restriction ;
                owl:allValuesFrom bibo:Book ;
                owl:onProperty terms:hasPart
              ] ;
      ns:term_status "stable" .

bibo:Report
      a       owl:Class ;
      rdfs:comment "A document describing an account or statement describing in detail an event, situation, or the like, usually as the result of observation, inquiry, etc.."@en ;
      rdfs:isDefinedBy "http://purl.org/ontology/bibo/"^^xsd:anyURI ;
      rdfs:label "Report"@en ;
      rdfs:subClassOf bibo:Document ;
      ns:term_status "stable" .

prism:number
      a       owl:DatatypeProperty ;
      owl:equivalentProperty
              bibo:locator .

bibo:Standard
      a       owl:Class ;
      rdfs:comment "A document describing a standard"@en ;
      rdfs:isDefinedBy "http://purl.org/ontology/bibo/"^^xsd:anyURI ;
      rdfs:label "Standard"@en ;
      rdfs:subClassOf bibo:Document ;
      ns:term_status "stable" .

bibo:LegalDocument
      a       owl:Class ;
      rdfs:comment "A legal document; for example, a court decision, a brief, and so forth."@en ;
      rdfs:isDefinedBy "http://purl.org/ontology/bibo/"^^xsd:anyURI ;
      rdfs:label "Legal Document"@en ;
      rdfs:subClassOf bibo:Document ;
      ns:term_status "stable" .

schema:localityName
      a       owl:DatatypeProperty ;
      skos:scopeNote "Used to name the locality of a publisher, an author, etc."@en .

prism:edition
      a       owl:DatatypeProperty ;
      owl:equivalentProperty
              bibo:edition .

bibo:Collection
      a       owl:Class ;
      rdfs:comment "A collection of Documents or Collections"@en ;
      rdfs:isDefinedBy "http://purl.org/ontology/bibo/"^^xsd:anyURI ;
      rdfs:label "Collection"@en ;
      rdfs:subClassOf
              [ a       owl:Restriction ;
                owl:allValuesFrom
                        [ a       owl:Class ;
                          owl:unionOf (bibo:Collection bibo:Document)
                        ] ;
                owl:onProperty terms:hasPart
              ] ;
      ns:term_status "stable" .

foaf:name
      a       owl:DatatypeProperty .

bibo:DocumentStatus
      a       owl:Class ;
      rdfs:comment "The status of the publication of a document."@en ;
      rdfs:isDefinedBy "http://purl.org/ontology/bibo/"^^xsd:anyURI ;
      rdfs:label "Document Status"@en ;
      ns:term_status "stable" .

terms:relation
      a       owl:ObjectProperty .

terms:rights
      a       owl:ObjectProperty ;
      skos:scopeNote "Used to describe rights related to a bibliographic resource."@en .

prism:startingPage
      a       owl:DatatypeProperty ;
      owl:equivalentProperty
              bibo:pageStart .

bibo:Legislation
      a       owl:Class ;
      rdfs:comment "A legal document proposing or enacting a law or a group of laws."@en ;
      rdfs:isDefinedBy "http://purl.org/ontology/bibo/"^^xsd:anyURI ;
      rdfs:label "Legislation"@en ;
      rdfs:subClassOf bibo:LegalDocument ;
      ns:term_status "unstable" .

prism:eIssn
      a       owl:DatatypeProperty ;
      owl:equivalentProperty
              bibo:eissn .

terms:language
      a       owl:ObjectProperty ;
      skos:scopeNote "Used to link a bibliographic resource to the language used to express it."@en .

bibo:pageEnd
      a       owl:DatatypeProperty ;
      rdfs:comment "Ending page number within a continuous page range."@en ;
      rdfs:domain bibo:Document ;
      rdfs:isDefinedBy "http://purl.org/ontology/bibo/"^^xsd:anyURI ;
      rdfs:label "page end"@en ;
      rdfs:range rdfs:Literal ;
      rdfs:subPropertyOf bibo:locator ;
      ns:term_status "stable" .

bibo:Webpage
      a       owl:Class ;
      rdfs:comment "A web page is an online document available (at least initially) on the world wide web. A web page is written first and foremost to appear on the web, as distinct from other online resources such as books, manuscripts or audio documents which use the web primarily as a distribution mechanism alongside other more traditional methods such as print."@en ;
      rdfs:isDefinedBy "http://purl.org/ontology/bibo/"^^xsd:anyURI ;
      rdfs:label "Webpage"@en ;
      rdfs:subClassOf bibo:Document ;
      ns:term_status "unstable" .

bibo:AudioDocument
      a       owl:Class ;
      rdfs:comment "An audio document; aka record."@en ;
      rdfs:isDefinedBy "http://purl.org/ontology/bibo/"^^xsd:anyURI ;
      rdfs:label "audio document"@en ;
      rdfs:subClassOf bibo:Document ;
      ns:term_status "stable" .

bibo:BookSection
      a       owl:Class ;
      rdfs:comment "A section of a book."@en ;
      rdfs:isDefinedBy "http://purl.org/ontology/bibo/"^^xsd:anyURI ;
      rdfs:label "Book Section"@en ;
      rdfs:subClassOf bibo:DocumentPart ;
      ns:term_status "unstable" .

bibo:LegalDecision
      a       owl:Class ;
      rdfs:comment "A document containing an authoritative determination (as a decree or judgment) made after consideration of facts or law."@en ;
      rdfs:isDefinedBy "http://purl.org/ontology/bibo/"^^xsd:anyURI ;
      rdfs:label "Decision"@en ;
      rdfs:subClassOf bibo:LegalCaseDocument ;
      ns:term_status "unstable" .

bibo:cites
      a       owl:ObjectProperty ;
      rdfs:comment """Relates a document to another document that is cited
by the first document as reference, comment, review, quotation or for
another purpose."""@en ;
      rdfs:domain bibo:Document ;
      rdfs:isDefinedBy "http://purl.org/ontology/bibo/"^^xsd:anyURI ;
      rdfs:label "cites"@en ;
      rdfs:range bibo:Document ;
      rdfs:subPropertyOf terms:references ;
      ns:term_status "unstable" .

bibo:court
      a       owl:ObjectProperty ;
      rdfs:comment "A court associated with a legal document; for example, that which issues a decision."@en ;
      rdfs:domain bibo:LegalDocument ;
      rdfs:isDefinedBy "http://purl.org/ontology/bibo/"^^xsd:anyURI ;
      rdfs:label "court"@en ;
      rdfs:range foaf:Organization ;
      ns:term_status "unstable" .

bibo:AudioVisualDocument
      a       owl:Class ;
      rdfs:comment "An audio-visual document; film, video, and so forth."@en ;
      rdfs:isDefinedBy "http://purl.org/ontology/bibo/"^^xsd:anyURI ;
      rdfs:label "audio-visual document"@en ;
      rdfs:subClassOf bibo:Document ;
      ns:term_status "stable" .

bibo:distributor
      a       owl:ObjectProperty ;
      rdfs:comment "Distributor of a document or a collection of documents."@en ;
      rdfs:domain
              [ a       owl:Class ;
                owl:unionOf (bibo:Collection bibo:Document)
              ] ;
      rdfs:isDefinedBy "http://purl.org/ontology/bibo/"^^xsd:anyURI ;
      rdfs:label "distributor"@en ;
      rdfs:range foaf:Agent ;
      ns:term_status "stable" .

bibo:Interview
      a       owl:Class ;
      rdfs:comment "A formalized discussion between two or more people."@en ;
      rdfs:isDefinedBy "http://purl.org/ontology/bibo/"^^xsd:anyURI ;
      rdfs:label "Interview"@en ;
      rdfs:subClassOf event:Event ;
      ns:term_status "stable" .

bibo:translationOf
      a       owl:ObjectProperty ;
      rdfs:comment "Relates a translated document to the original document."@en ;
      rdfs:domain bibo:Document ;
      rdfs:isDefinedBy "http://purl.org/ontology/bibo/"^^xsd:anyURI ;
      rdfs:label "translation of"@en ;
      rdfs:range bibo:Document ;
      rdfs:subPropertyOf terms:isVersionOf ;
      ns:term_status "stable" .

terms:description
      a       owl:AnnotationProperty , owl:DatatypeProperty ;
      skos:scopeNote "Used to describe a bibliographic resource."@en .

bibo:Quote
      a       owl:Class ;
      rdfs:comment "An excerpted collection of words."@en ;
      rdfs:isDefinedBy "http://purl.org/ontology/bibo/"^^xsd:anyURI ;
      rdfs:label "Quote"@en ;
      rdfs:subClassOf bibo:Excerpt ;
      ns:term_status "stable" .

bibo:producer
      a       owl:ObjectProperty ;
      rdfs:comment "Producer of a document or a collection of documents."@en ;
      rdfs:domain
              [ a       owl:Class ;
                owl:unionOf (bibo:Collection bibo:Document)
              ] ;
      rdfs:isDefinedBy "http://purl.org/ontology/bibo/"^^xsd:anyURI ;
      rdfs:label "producer"@en ;
      rdfs:range foaf:Agent ;
      ns:term_status "stable" .

bibo:performer
      a       owl:ObjectProperty ;
      rdfs:domain bibo:Performance ;
      rdfs:isDefinedBy "http://purl.org/ontology/bibo/"^^xsd:anyURI ;
      rdfs:label "performer" ;
      rdfs:range foaf:Agent ;
      rdfs:subPropertyOf terms:contributor ;
      ns:term_status "stable" .

bibo:affirmedBy
      a       owl:ObjectProperty ;
      rdfs:comment "A legal decision that affirms a ruling."@en ;
      rdfs:domain bibo:LegalDecision ;
      rdfs:isDefinedBy "http://purl.org/ontology/bibo/"^^xsd:anyURI ;
      rdfs:range bibo:LegalDecision ;
      rdfs:subPropertyOf bibo:subsequentLegalDecision .

bibo:LegalCaseDocument
      a       owl:Class ;
      rdfs:comment "A document accompanying a legal case."@en ;
      rdfs:isDefinedBy "http://purl.org/ontology/bibo/"^^xsd:anyURI ;
      rdfs:label "Legal Case Document"@en ;
      rdfs:subClassOf bibo:LegalDocument ;
      ns:term_status "unstable" .

bibo:PersonalCommunicationDocument
      a       owl:Class ;
      rdfs:comment "A personal communication manifested in some document."@en ;
      rdfs:isDefinedBy "http://purl.org/ontology/bibo/"^^xsd:anyURI ;
      rdfs:label "Personal Communication Document"@en ;
      rdfs:subClassOf bibo:Document ;
      ns:term_status "stable" .

bibo:numVolumes
      a       owl:DatatypeProperty ;
      rdfs:comment "The number of volumes contained in a collection of documents (usually a series, periodical, etc.)."@en ;
      rdfs:domain bibo:Collection ;
      rdfs:isDefinedBy "http://purl.org/ontology/bibo/"^^xsd:anyURI ;
      rdfs:label "number of volumes"@en ;
      rdfs:range rdfs:Literal ;
      ns:term_status "stable" .

prism:volume
      a       owl:DatatypeProperty ;
      owl:equivalentProperty
              bibo:volume .

foaf:family_name
      a       owl:DatatypeProperty ;
      skos:scopeNote "This is the property we choose to use to describe the family name of a person related to a bibliographic resource."@en .

bibo:Series
      a       owl:Class ;
      rdfs:comment "A loose, thematic, collection of Documents, often Books."@en ;
      rdfs:isDefinedBy "http://purl.org/ontology/bibo/"^^xsd:anyURI ;
      rdfs:label "Series"@en ;
      rdfs:subClassOf bibo:Collection ;
      rdfs:subClassOf
              [ a       owl:Restriction ;
                owl:allValuesFrom bibo:Document ;
                owl:onProperty terms:hasPart
              ] ;
      ns:term_status "stable" .

bibo:translator
      a       owl:ObjectProperty ;
      rdfs:comment "A person who translates written document from one language to another."@en ;
      rdfs:domain
              [ a       owl:Class ;
                owl:unionOf (bibo:Collection bibo:Document)
              ] ;
      rdfs:isDefinedBy "http://purl.org/ontology/bibo/"^^xsd:anyURI ;
      rdfs:label "translator" ;
      rdfs:range foaf:Agent ;
      rdfs:subPropertyOf terms:contributor ;
      ns:term_status "stable" .

bibo:editorList
      a       owl:ObjectProperty ;
      rdfs:comment "An ordered list of editors. Normally, this list is seen as a priority list that order editors by importance."@en ;
      rdfs:domain bibo:Document ;
      rdfs:isDefinedBy "http://purl.org/ontology/bibo/"^^xsd:anyURI ;
      rdfs:label "list of editors"@en ;
      rdfs:range
              [ a       owl:Class ;
                owl:unionOf (rdf:List rdf:Seq)
              ] ;
      rdfs:subPropertyOf bibo:contributorList ;
      ns:term_status "stable" .

bibo:subsequentLegalDecision
      a       owl:ObjectProperty ;
      rdfs:comment "A legal decision on appeal that takes action on a case (affirming it, reversing it, etc.)."@en ;
      rdfs:domain bibo:LegalDecision ;
      rdfs:isDefinedBy "http://purl.org/ontology/bibo/"^^xsd:anyURI ;
      rdfs:range bibo:LegalDecision ;
      rdfs:subPropertyOf terms:isReferencedBy .

terms:subject
      a       owl:ObjectProperty ;
      skos:scopeNote "Used to describe the subject of a bibliographic resource."@en .

bibo:coden
      a       owl:DatatypeProperty ;
      rdfs:domain
              [ a       owl:Class ;
                owl:unionOf (bibo:Collection bibo:Document)
              ] ;
      rdfs:range rdfs:Literal ;
      rdfs:subPropertyOf bibo:identifier .

bibo:presents
      a       owl:ObjectProperty ;
      rdfs:comment "Relates an event to associated documents; for example, conference to a paper."@en ;
      rdfs:domain bibo:Event ;
      rdfs:isDefinedBy "http://purl.org/ontology/bibo/"^^xsd:anyURI ;
      rdfs:label "presented at"@en ;
      rdfs:range bibo:Document ;
      rdfs:subPropertyOf event:product ;
      owl:inverseOf bibo:presentedAt ;
      ns:term_status "unstable" .

bibo:citedBy
      a       owl:ObjectProperty ;
      rdfs:comment """Relates a document to another document that cites the
first document."""@en ;
      rdfs:domain bibo:Document ;
      rdfs:isDefinedBy "http://purl.org/ontology/bibo/"^^xsd:anyURI ;
      rdfs:label "cited by"@en ;
      rdfs:range bibo:Document ;
      owl:inverseOf bibo:cites ;
      ns:term_status "unstable" .

bibo:contributorList
      a       owl:ObjectProperty ;
      rdfs:comment "An ordered list of contributors. Normally, this list is seen as a priority list that order contributors by importance."@en ;
      rdfs:domain bibo:Document ;
      rdfs:isDefinedBy "http://purl.org/ontology/bibo/"^^xsd:anyURI ;
      rdfs:label "list of contributors"@en ;
      rdfs:range
              [ a       owl:Class ;
                owl:unionOf (rdf:List rdf:Seq)
              ] ;
      ns:term_status "stable" .

bibo:Manual
      a       owl:Class ;
      rdfs:comment "A small reference book, especially one giving instructions."@en ;
      rdfs:isDefinedBy "http://purl.org/ontology/bibo/"^^xsd:anyURI ;
      rdfs:label "Manual"@en ;
      rdfs:subClassOf bibo:Document ;
      ns:term_status "unstable" .

bibo:locator
      a       owl:DatatypeProperty ;
      rdfs:comment "A description (often numeric) that locates an item within a containing document or collection."@en ;
      rdfs:domain bibo:Document ;
      rdfs:isDefinedBy "http://purl.org/ontology/bibo/"^^xsd:anyURI ;
      rdfs:label "locator"@en ;
      rdfs:range rdfs:Literal ;
      ns:term_status "stable" .

status:peerReviewed
      a       bibo:DocumentStatus , owl:Thing , owl:NamedIndividual ;
      rdfs:comment "The process by which articles are chosen to be included in a refereed journal. An editorial board consisting of experts in the same field as the author review the article and decide if it is authoritative enough for publication."@en ;
      rdfs:label "peer reviewed"@en ;
      ns:term_status "stable" .

prism:doi
      a       owl:DatatypeProperty ;
      owl:equivalentProperty
              bibo:doi .

bibo:Article
      a       owl:Class ;
      rdfs:comment "A written composition in prose, usually nonfiction, on a specific topic, forming an independent part of a book or other publication, as a newspaper or magazine."@en ;
      rdfs:isDefinedBy "http://purl.org/ontology/bibo/"^^xsd:anyURI ;
      rdfs:label "Article"@en ;
      rdfs:subClassOf bibo:Document ;
      ns:term_status "stable" .

foaf:Image
      a       owl:Class .

bibo:eissn
      a       owl:DatatypeProperty ;
      rdfs:domain bibo:Collection ;
      rdfs:range rdfs:Literal ;
      rdfs:subPropertyOf bibo:identifier .

bibo:isbn
      a       owl:DatatypeProperty ;
      rdfs:subPropertyOf bibo:identifier .

bibo:Statute
      a       owl:Class ;
      rdfs:comment "A bill enacted into law."@en ;
      rdfs:isDefinedBy "http://purl.org/ontology/bibo/"^^xsd:anyURI ;
      rdfs:label "Statute"@en ;
      rdfs:subClassOf bibo:Legislation ;
      ns:term_status "stable" .

bibo:degree
      a       owl:ObjectProperty ;
      rdfs:comment "The thesis degree."@en ;
      rdfs:domain bibo:Thesis ;
      rdfs:isDefinedBy "http://purl.org/ontology/bibo/"^^xsd:anyURI ;
      rdfs:label "degree"@en ;
      rdfs:range bibo:ThesisDegree ;
      ns:term_status "unstable" ;
      skos:editorialNote "We are not defining, using an enumeration, the range of the bibo:degree to the defined list of bibo:ThesisDegree. We won't do it because we want people to be able to define new degress if needed by some special usecases. Creating such an enumeration would restrict this to happen."@en .

terms:Agent
      a       owl:Class ;
      owl:equivalentClass foaf:Agent ;
      skos:editorialNote """BIBO assert that a dcterms:Agent is an equivalent class to foaf:Agent.
This means that all the individuals belonging to the foaf:Agent class
also belongs to the dcterms:Agent class. This way, dcterms:contributor
can be used on foaf:Person, foaf:Organization, foaf:Agent and foaf:Group.
Even if this link is not done in neither the FOAF nor the DCTERMS ontologies this is a wide spread fact that is asserted by BIBO."""@en .

bibo:Proceedings
      a       owl:Class ;
      rdfs:comment "A compilation of documents published from an event, such as a conference."@en ;
      rdfs:isDefinedBy "http://purl.org/ontology/bibo/"^^xsd:anyURI ;
      rdfs:label "Proceedings"@en ;
      rdfs:subClassOf bibo:Book ;
      ns:term_status "unstable" .

bibo:presentedAt
      a       owl:ObjectProperty ;
      rdfs:comment "Relates a document to an event; for example, a paper to a conference."@en ;
      rdfs:domain bibo:Document ;
      rdfs:isDefinedBy "http://purl.org/ontology/bibo/"^^xsd:anyURI ;
      rdfs:label "presented at"@en ;
      rdfs:range bibo:Event ;
      rdfs:subPropertyOf event:produced_in ;
      ns:term_status "unstable" .

bibo:DocumentPart
      a       owl:Class ;
      rdfs:comment "a distinct part of a larger document or collected document."@en ;
      rdfs:isDefinedBy "http://purl.org/ontology/bibo/"^^xsd:anyURI ;
      rdfs:label "document part"@en ;
      rdfs:subClassOf bibo:Document ;
      rdfs:subClassOf
              [ a       owl:Restriction ;
                owl:maxCardinality "1"^^xsd:nonNegativeInteger ;
                owl:onProperty terms:isPartOf
              ] ;
      ns:term_status "unstable" .

bibo:Book
      a       owl:Class ;
      rdfs:comment "A written or printed work of fiction or nonfiction, usually on sheets of paper fastened or bound together within covers."@en ;
      rdfs:isDefinedBy "http://purl.org/ontology/bibo/"^^xsd:anyURI ;
      rdfs:label "Book"@en ;
      rdfs:subClassOf bibo:Document ;
      ns:term_status "stable" .

status:forthcoming
      a       bibo:DocumentStatus , owl:Thing , owl:NamedIndividual ;
      rdfs:comment "Document to be published"@en ;
      rdfs:label "forthcoming"@en ;
      ns:term_status "stable" .

foaf:Organization
      a       owl:Class ;
      skos:scopeNote "Ued to describe an organization related to bibliographic items such as a publishing company, etc."@en .

bibo:interviewee
      a       owl:ObjectProperty ;
      rdfs:comment "An agent that is interviewed by another agent."@en ;
      rdfs:domain foaf:Agent ;
      rdfs:isDefinedBy "http://purl.org/ontology/bibo/"^^xsd:anyURI ;
      rdfs:label "interviewee" ;
      rdfs:range foaf:Agent ;
      rdfs:subPropertyOf terms:contributor ;
      ns:term_status "stable" .

prism:isbn
      a       owl:DatatypeProperty ;
      owl:equivalentProperty
              bibo:isbn .

bibo:transcriptOf
      a       owl:ObjectProperty ;
      rdfs:comment "Relates a document to some transcribed original."@en ;
      rdfs:domain bibo:Document ;
      rdfs:isDefinedBy "http://purl.org/ontology/bibo/"^^xsd:anyURI ;
      rdfs:label "transcript of"@en ;
      rdfs:range rdfs:Resource ;
      rdfs:subPropertyOf terms:relation ;
      ns:term_status "unstable" .

prism:issue
      a       owl:DatatypeProperty ;
      owl:equivalentProperty
              bibo:issue .

bibo:issuer
      a       owl:ObjectProperty ;
      rdfs:comment "An entity responsible for issuing often informally published documents such as press releases, reports, etc." ;
      rdfs:domain
              [ a       owl:Class ;
                owl:unionOf (bibo:Collection bibo:Document)
              ] ;
      rdfs:isDefinedBy "http://purl.org/ontology/bibo/"^^xsd:anyURI ;
      rdfs:label "issuer" ;
      rdfs:range foaf:Agent ;
      rdfs:subPropertyOf terms:publisher ;
      ns:term_status "unstable" .

bibo:shortTitle
      a       owl:DatatypeProperty ;
      rdfs:comment "The abbreviation of a title."@en ;
      rdfs:domain bibo:Document ;
      rdfs:isDefinedBy "http://purl.org/ontology/bibo/"^^xsd:anyURI ;
      rdfs:label "short title"@en ;
      rdfs:range rdfs:Literal ;
      ns:term_status "stable" .

bibo:numPages
      a       owl:DatatypeProperty ;
      rdfs:comment "The number of pages contained in a document"@en ;
      rdfs:domain bibo:Document ;
      rdfs:isDefinedBy "http://purl.org/ontology/bibo/"^^xsd:anyURI ;
      rdfs:label "number of pages"@en ;
      rdfs:range rdfs:Literal ;
      ns:term_status "stable" .

rdf:Seq
      a       owl:Class .

bibo:oclcnum
      a       owl:DatatypeProperty ;
      rdfs:domain
              [ a       owl:Class ;
                owl:unionOf (bibo:Collection bibo:Document)
              ] ;
      rdfs:range rdfs:Literal ;
      rdfs:subPropertyOf bibo:identifier .

bibo:isbn10
      a       owl:DatatypeProperty ;
      rdfs:domain
              [ a       owl:Class ;
                owl:unionOf (bibo:Collection bibo:Document)
              ] ;
      rdfs:range rdfs:Literal ;
      rdfs:subPropertyOf bibo:isbn .

bibo:Hearing
      a       owl:Class ;
      rdfs:comment "An instance or a session in which testimony and arguments are presented, esp. before an official, as a judge in a lawsuit."@en ;
      rdfs:isDefinedBy "http://purl.org/ontology/bibo/"^^xsd:anyURI ;
      rdfs:label "Hearing"@en ;
      rdfs:subClassOf event:Event ;
      ns:term_status "stable" .

bibo:editor
      a       owl:ObjectProperty ;
      rdfs:comment "A person having managerial and sometimes policy-making responsibility for the editorial part of a publishing firm or of a newspaper, magazine, or other publication."@en ;
      rdfs:domain
              [ a       owl:Class ;
                owl:unionOf (bibo:Collection bibo:Document)
              ] ;
      rdfs:isDefinedBy "http://purl.org/ontology/bibo/"^^xsd:anyURI ;
      rdfs:label "editor" ;
      rdfs:range foaf:Agent ;
      rdfs:subPropertyOf terms:contributor ;
      ns:term_status "stable" .

foaf:Document
      a       owl:Class .

owl:Thing
      a       owl:Class .

bibo:Brief
      a       owl:Class ;
      rdfs:comment "A written argument submitted to a court."@en ;
      rdfs:isDefinedBy "http://purl.org/ontology/bibo/"^^xsd:anyURI ;
      rdfs:label "Brief"@en ;
      rdfs:subClassOf bibo:LegalCaseDocument ;
      ns:term_status "unstable" .

bibo:reproducedIn
      a       owl:ObjectProperty ;
      rdfs:comment "The resource in which another resource is reproduced."@en ;
      rdfs:domain bibo:Document ;
      rdfs:isDefinedBy "http://purl.org/ontology/bibo/"^^xsd:anyURI ;
      rdfs:range bibo:Document ;
      rdfs:subPropertyOf terms:isPartOf ;
      ns:term_status "unstable" .

terms:issued
      a       owl:DatatypeProperty ;
      rdfs:subPropertyOf terms:date ;
      skos:scopeNote "Used to describe the issue date of a bibliographic resource"@en .

bibo:content
      a       owl:DatatypeProperty ;
      rdfs:comment "This property is for a plain-text rendering of the content of a Document. While the plain-text content of an entire document could be described by this property."@en ;
      rdfs:domain bibo:Document ;
      rdfs:isDefinedBy "http://purl.org/ontology/bibo/"^^xsd:anyURI ;
      rdfs:label "content"@en ;
      rdfs:range rdfs:Literal ;
      owl:deprecated "true"^^xsd:boolean ;
      ns:term_status "unstable" ;
      skos:historyNote "bibo:content has been deprecated; we recommend to use \"rdf:value\" for this purpose. Here is the rational behind this choice: http://www.w3.org/TR/2004/REC-rdf-primer-20040210/#rdfvalue"@en .

bibo:asin
      a       owl:DatatypeProperty ;
      rdfs:domain
              [ a       owl:Class ;
                owl:unionOf (bibo:Collection bibo:Document)
              ] ;
      rdfs:range rdfs:Literal ;
      rdfs:subPropertyOf bibo:identifier .

bibo:suffixName
      a       owl:DatatypeProperty ;
      rdfs:comment "The suffix of a name"@en ;
      rdfs:domain foaf:Agent ;
      rdfs:isDefinedBy "http://purl.org/ontology/bibo/"^^xsd:anyURI ;
      rdfs:label "suffix name"@en ;
      rdfs:range rdfs:Literal ;
      ns:term_status "stable" .

bibo:bdarcus
      a       foaf:Person , owl:Thing , owl:NamedIndividual ;
      rdfs:isDefinedBy "http://purl.org/ontology/bibo/"^^xsd:anyURI ;
      rdfs:seeAlso "http://purl.org/net/darcusb/info#me"^^xsd:anyURI ;
      foaf:name "Bruce D'Arcus" .

event:Event
      a       owl:Class ;
      skos:scopeNote "Used to describe bibliographic related events such as conferences, hearing, etc."@en .

bibo:
      a       owl:Ontology ;
      terms:creator bibo:fgiasson , bibo:bdarcus ;
      terms:description """The Bibliographic Ontology describes
bibliographic things on the semantic Web in RDF.  This ontology can be
used as a citation ontology, as a document classification ontology, or
simply as a way to describe any kind of document in RDF. It has been
inspired by many existing document description metadata formats, and
can be used as a common ground for converting other bibliographic data
sources."""@en ;
      terms:title "The Bibliographic Ontology" ;
      owl:versionInfo "http://purl.org/ontology/bibo/1.3/" .

terms:date
      a       owl:DatatypeProperty ;
      skos:scopeNote "Use to link a bibliographic item to the date of an event. Check dcterms:created and other for proper specializations for this property"@en .

bibo:Image
      a       owl:Class ;
      rdfs:comment "A document that presents visual or diagrammatic information."@en ;
      rdfs:isDefinedBy "http://purl.org/ontology/bibo/"^^xsd:anyURI ;
      rdfs:label "Image"@en ;
      rdfs:subClassOf bibo:Document ;
      owl:equivalentClass foaf:Image ;
      ns:term_status "stable" .

bibo:organizer
      a       owl:ObjectProperty ;
      rdfs:comment "The organizer of an event; includes conference organizers, but also government agencies or other bodies that are responsible for conducting hearings."@en ;
      rdfs:domain event:Event ;
      rdfs:isDefinedBy "http://purl.org/ontology/bibo/"^^xsd:anyURI ;
      rdfs:label "organizer"@en ;
      rdfs:range foaf:Agent ;
      ns:term_status "unstable" .

bibo:isbn13
      a       owl:DatatypeProperty ;
      rdfs:domain
              [ a       owl:Class ;
                owl:unionOf (bibo:Collection bibo:Document)
              ] ;
      rdfs:range rdfs:Literal ;
      rdfs:subPropertyOf bibo:isbn .

bibo:uri
      a       owl:DatatypeProperty ;
      rdfs:comment "Universal Resource Identifier of a document"@en ;
      rdfs:domain
              [ a       owl:Class ;
                owl:unionOf (bibo:Collection bibo:Document)
              ] ;
      rdfs:isDefinedBy "http://purl.org/ontology/bibo/"^^xsd:anyURI ;
      rdfs:label "uri"@en ;
      rdfs:range rdfs:Literal ;
      rdfs:subPropertyOf bibo:identifier ;
      ns:term_status "stable" .

bibo:edition
      a       owl:DatatypeProperty ;
      rdfs:comment "The name defining a special edition of a document. Normally its a literal value composed of a version number and words."@en ;
      rdfs:domain bibo:Document ;
      rdfs:isDefinedBy "http://purl.org/ontology/bibo/"^^xsd:anyURI ;
      rdfs:label "edition"@en ;
      rdfs:range rdfs:Literal ;
      ns:term_status "stable" .

bibo:Document
      a       owl:Class ;
      rdfs:comment "A document (noun) is a bounded physical representation of body of information designed with the capacity (and usually intent) to communicate. A document may manifest symbolic, diagrammatic or sensory-representational information."@en ;
      rdfs:isDefinedBy "http://purl.org/ontology/bibo/"^^xsd:anyURI ;
      rdfs:label "Document"@en ;
      owl:equivalentClass foaf:Document ;
      ns:term_status "stable" .

bibo:Bill
      a       owl:Class ;
      rdfs:comment "Draft legislation presented for discussion to a legal body."@en ;
      rdfs:isDefinedBy "http://purl.org/ontology/bibo/"^^xsd:anyURI ;
      rdfs:label "Bill"@en ;
      rdfs:subClassOf bibo:Legislation ;
      ns:term_status "stable" .

bibo:AcademicArticle
      a       owl:Class ;
      rdfs:comment "A scholarly academic article, typically published in a journal."@en ;
      rdfs:isDefinedBy "http://purl.org/ontology/bibo/"^^xsd:anyURI ;
      rdfs:label "Academic Article"@en ;
      rdfs:subClassOf bibo:Article ;
      ns:term_status "stable" .

bibo:ReferenceSource
      a       owl:Class ;
      rdfs:comment "A document that presents authoritative reference information, such as a dictionary or encylopedia ."@en ;
      rdfs:isDefinedBy "http://purl.org/ontology/bibo/"^^xsd:anyURI ;
      rdfs:label "Reference Source"@en ;
      rdfs:subClassOf bibo:Document ;
      ns:term_status "unstable" .

bibo:eanucc13
      a       owl:DatatypeProperty ;
      rdfs:domain
              [ a       owl:Class ;
                owl:unionOf (bibo:Collection bibo:Document)
              ] ;
      rdfs:range rdfs:Literal ;
      rdfs:subPropertyOf bibo:identifier .

bibo:EditedBook
      a       owl:Class ;
      rdfs:comment "An edited book."@en ;
      rdfs:isDefinedBy "http://purl.org/ontology/bibo/"^^xsd:anyURI ;
      rdfs:label "Edited Book"@en ;
      rdfs:subClassOf bibo:CollectedDocument ;
      ns:term_status "stable" .

bibo:PersonalCommunication
      a       owl:Class ;
      rdfs:comment "A communication between an agent and one or more specific recipients."@en ;
      rdfs:isDefinedBy "http://purl.org/ontology/bibo/"^^xsd:anyURI ;
      rdfs:label "Personal Communication"@en ;
      rdfs:subClassOf event:Event ;
      ns:term_status "stable" .

bibo:gtin14
      a       owl:DatatypeProperty ;
      rdfs:domain
              [ a       owl:Class ;
                owl:unionOf (bibo:Collection bibo:Document)
              ] ;
      rdfs:range rdfs:Literal ;
      rdfs:subPropertyOf bibo:identifier .

bibo:doi
      a       owl:DatatypeProperty ;
      rdfs:domain
              [ a       owl:Class ;
                owl:unionOf (bibo:Collection bibo:Document)
              ] ;
      rdfs:range rdfs:Literal ;
      rdfs:subPropertyOf bibo:identifier .

bibo:shortDescription
      a       owl:DatatypeProperty ;
      rdfs:domain bibo:Document ;
      rdfs:range rdfs:Literal .

bibo:status
      a       owl:ObjectProperty ;
      rdfs:comment "The publication status of (typically academic) content."@en ;
      rdfs:domain bibo:Document ;
      rdfs:isDefinedBy "http://purl.org/ontology/bibo/"^^xsd:anyURI ;
      rdfs:label "status"@en ;
      rdfs:range bibo:DocumentStatus ;
      ns:term_status "stable" ;
      skos:editorialNote "We are not defining, using an enumeration, the range of the bibo:status to the defined list of bibo:DocumentStatus. We won't do it because we want people to be able to define new status if needed by some special usecases. Creating such an enumeration would restrict this to happen."@en .

event:place
      a       owl:ObjectProperty ;
      skos:scopeNote "Used to relate an event such as a conference to the geographical place where it happens, for example Paris."@en .
